elo-coq/Properties.v
@@ -1,4 +1,5 @@
 From Coq Require Import Arith.Arith.
+From Coq Require Import Lists.List.
 
 From Elo Require Export Array.
 From Elo Require Export Map.
@@ -11,7 +12,9 @@ Ltac splits n :=
   | S ?n' => split; [| splits n']
   end.
 
-(* Determinism *)
+(* ------------------------------------------------------------------------- *)
+(* Determinism ------------------------------------------------------------- *)
+(* ------------------------------------------------------------------------- *)
 
 Lemma value_does_not_step : forall m m' v t eff,
   value v -> ~ (m / v --> eff / m' / t).
@@ -59,13 +62,15 @@ Proof.
     ].
 Qed.
 
-(* Progress, Preservation & Soundness *)
+(* ------------------------------------------------------------------------- *)
+(* Progress, Preservation & Soundness -------------------------------------- *)
+(* ------------------------------------------------------------------------- *)
 
 Definition well_typed_memory (mt : list typ) (m : mem) :=
   length mt = length m /\
   (forall i, mt / empty |-- (get_tm m i) is (get_typ mt i)).
 
-Inductive extends' : list typ -> list typ -> Prop :=
+Inductive extends' {A} : list A -> list A -> Prop :=
   | extends_nil : forall mt,
     extends' mt nil
   | extends_cons : forall x mt mt',
@@ -89,7 +94,7 @@ Proof.
     + unfold get_typ, get. simpl in *. eauto using Lt.lt_S_n.
 Qed.
 
-Lemma extends_length : forall i mt mt',
+Lemma extends_length : forall {A} i (mt mt' : list A),
   i < length mt' ->
   mt extends mt' ->
   i < length mt.
@@ -103,16 +108,16 @@ Proof.
     eauto using PeanoNat.Nat.lt_0_succ, Lt.lt_n_S, Lt.lt_S_n.
 Qed.
 
-Lemma extends_add : forall mt x,
+Lemma extends_add : forall {A} (mt : list A) x,
   (add mt x) extends mt.
 Proof.
-  induction mt; eauto using extends'.
+  induction mt; eauto using @extends'.
 Qed.
 
-Lemma extends_refl : forall mt,
+Lemma extends_refl : forall {A} (mt : list A),
   mt extends mt.
 Proof.
-  induction mt; auto using extends'.
+  induction mt; auto using @extends'.
 Qed.
 
 Lemma memory_weakening : forall mt mt' Gamma t T, 
@@ -177,7 +182,7 @@ Lemma update_safe_includes_safe_update : forall Gamma id T,
 Proof.
   unfold Map.includes', update, Map.update', safe. intros *.
   destruct String.eqb; trivial.
-  destruct safe_type_bool; trivial.
+  destruct is_safe_type; trivial.
   intros F. inversion F.
 Qed.
 
@@ -330,6 +335,11 @@ Proof.
     try (eexists; eexists; eauto using step; fail).
     destruct Hv; inversion Htype1; subst.
     eexists; eexists; eauto using step.
+(*
+  - destruct (IHHtype1 eq_refl) as [Hv | [? [? [? ?]]]];
+    destruct (IHHtype2 eq_refl) as [?  | [? [? [? ?]]]];
+    eexists; eexists; eauto using step.
+*)
 Qed.
 
 Definition normal_form m t : Prop :=
@@ -356,4 +366,233 @@ Proof.
     eauto using preservation. decompose record Hpreservation.
     assert (Hprogress : value t \/ exists m' t' eff, m / t --> eff / m' / t').
     eauto using progress. destruct Hprogress; eauto.
+Qed.
+
+(* ------------------------------------------------------------------------- *)
+(* Concurrent Progress, Preservation & Soundness --------------------------- *)
+(* ------------------------------------------------------------------------- *)
+
+Definition empties (threads : list tm) :=
+  List.repeat (@empty typ) (length threads).
+
+Definition get_ctx := get (@empty typ).
+
+Definition well_typed_threads mt Gammas threads := forall i,
+  length Gammas = length threads ->
+  exists T, mt / (get_ctx Gammas i) |-- (get_tm threads i) is T.
+
+Definition finished threads :=
+  forall i, value (get_tm threads i).
+
+
+
+Lemma aux1 : forall t ts i,
+  get_tm (t :: ts) (S i) = get_tm ts i.
+Proof.
+  unfold get_tm, get. intros *. reflexivity.
+Qed.
+
+Lemma aux3 : forall {A B} (x : A) xs (y : B) ys,
+  length xs = length ys -> length (x :: xs) = length (y :: ys).
+Proof.
+  intros * H. simpl. f_equal. assumption.
+Qed.
+
+Lemma aux2 : forall Gamma Gammas ths th mt,
+  well_typed_threads mt (Gamma :: Gammas) (th :: ths) ->
+  well_typed_threads mt Gammas ths.
+Proof.
+  unfold well_typed_threads. simpl.
+  intros *. intros H i Hlen.
+  eapply eq_S in Hlen.
+  specialize (H (S i) Hlen) as [T H].
+  exists T. rewrite aux1 in H. assumption.
+Qed.
+
+Lemma aux4 : forall (th : tm) ths,
+  empties (th :: ths) = empty :: empties (ths).
+Proof.
+Admitted.
+
+Lemma aux5 : forall m m' th ths ths',
+  m / ths ==> m' / ths' ->
+  m / (th :: ths) ==> m' / (th :: ths').
+Proof.
+  intros * H. induction H.
+  - apply (CST_None (S i) _ _ _ (th :: threads)).
+    unfold get_tm. rewrite get_S_i. assumption.
+  - apply (CST_Spawn (S i) _ m' _ _ (th :: threads)).
+    + simpl. auto using lt_n_S.
+    + unfold get_tm. rewrite get_S_i. assumption.
+Qed.
+
+Lemma aux6 : forall (l : list tm),
+  S (length (empties l)) = S (length l).
+Proof.
+Admitted.
+
+Lemma empties_length : forall threads,
+  length (empties threads) = length threads.
+Proof.
+Admitted.
+
+Lemma empties_returns_empty : forall threads i,
+  get_ctx (empties threads) i = empty.
+Proof.
+  intros *. unfold get_ctx, empties. generalize dependent i.
+  induction threads as [| ? ? IH]; intros i; destruct i; trivial.
+  apply IH.
+Qed.
+
+Lemma set_preserves_empties : forall threads i t,
+  empties (set threads i t) = empties threads.
+Proof.
+  intros. unfold empties. rewrite <- set_preserves_length. reflexivity.
+Qed.
+
+(* TODO : move to Array *)
+Lemma get_default : forall {A} d (l : list A) i,
+  length l <= i -> get d l i = d.
+Proof.
+  intros ? ? l. induction l as [| ? ? IH]; intros i Hlen; destruct i; trivial.
+  - apply Nat.nle_succ_0 in Hlen. contradiction.
+  - simpl in *. apply le_S_n in Hlen. apply (IH i Hlen).
+Qed.
+
+(* TODO : move to Array *)
+Lemma get_set_default : forall {A} d (l : list A) i a,
+  length l <= i ->
+  get d (set l i a) i = d.
+Proof.
+  intros * Hlen.
+  erewrite set_preserves_length in Hlen.
+  eauto using get_default.
+Qed.
+
+(* TODO : move to Array *)
+Lemma add_set_comm : forall {A} (l : list A) i a1 a2,
+  i < length l ->
+  add (set l i a1) a2 = set (add l a2) i a1.
+Proof.
+  unfold add.
+  intros ? l. induction l as [| ? ? IH]; intros * H.
+  - destruct i eqn:E.
+    + inversion H.
+    + reflexivity.
+  - simpl in *. destruct i eqn:E.
+    + reflexivity.
+    + apply lt_S_n in H. rewrite <- (IH n a1 a2 H). reflexivity.
+Qed.
+
+Lemma step_preserves_well_typed_threads : forall mt m m' eff threads t i,
+  m / get_tm threads i --> eff / m' / t ->
+  well_typed_memory mt m ->
+  well_typed_threads mt (empties threads) threads ->
+  exists mt',
+    mt' extends mt /\
+    well_typed_threads mt' (empties (set threads i t)) (set threads i t) /\
+    well_typed_memory mt' m'.
+Proof.
+  intros * Hstep Hmem Hctype.
+  destruct (Hctype i (empties_length threads)) as [T Htype].
+  rewrite empties_returns_empty in Htype.
+  assert (Preservation : exists mt',
+            mt' extends mt /\
+            mt' / empty |-- t is T /\
+            well_typed_memory mt' m').
+  { eauto using preservation. }
+  destruct Preservation as [? [? [? ?]]].
+  eexists. splits 3; eauto.
+  intros i' ?. rewrite empties_returns_empty. unfold get_tm.
+  destruct (i =? i') eqn:E.
+  + apply Nat.eqb_eq in E. subst.
+    destruct (le_lt_dec (length threads) i').
+    * rewrite get_set_default; trivial. exists TY_Void. apply T_Nil.
+    * rewrite get_set_involutive; trivial. exists T. eauto.
+  + apply Nat.eqb_neq in E. apply not_eq_sym in E.
+    rewrite get_set_i_neq_j; trivial.
+    destruct (le_lt_dec (length threads) i').
+    * rewrite get_default; trivial. exists TY_Void. apply T_Nil.
+    * specialize (Hctype i' (empties_length threads)) as [? ?].
+      unfold get_tm in *.
+      rewrite empties_returns_empty in *.
+      eexists. eauto using memory_weakening.
+Qed.
+
+Lemma spawn_preserves_well_typed_threads : forall mt mt' threads block T,
+  mt' extends mt ->
+  mt / empty |-- block is T ->
+  well_typed_threads mt (empties threads) threads ->
+  well_typed_threads mt' (empties (add threads block)) (add threads block).
+Proof.
+  intros * Hext Htype Hctype i Hlen.
+  destruct (lt_eq_lt_dec i (length threads)) as [[? | ?] | ?].
+  - specialize (Hctype i (empties_length threads)) as [T' Htype'].
+    exists T'. unfold get_tm. rewrite get_add_lt; trivial.
+    rewrite empties_returns_empty in *. eauto using memory_weakening.
+  - exists T. unfold get_tm. subst. rewrite get_add_last.
+    rewrite empties_returns_empty in *. eauto using memory_weakening.
+  - unfold get_tm. rewrite get_add_gt; trivial.
+    rewrite empties_returns_empty.
+    exists TY_Void. apply T_Nil.
+Qed.
+
+Lemma spawn_block_has_type: forall mt m m' t t' block T,
+  mt / empty |-- t is T ->
+  m / t --> EF_Spawn block / m' / t' ->
+  exists B, mt / empty |-- block is B.
+Proof.
+  intros ? ? ? t. induction t; intros * Htype Hstep;
+  inversion Hstep; inversion Htype; eauto. subst.
+  eexists. eauto.
+Qed.
+
+Theorem cpreservation : forall threads threads' m m' mt,
+  well_typed_threads mt (empties threads) threads ->
+  well_typed_memory mt m ->
+  m / threads ==> m' / threads' ->
+  exists mt',
+    mt' extends mt /\
+    well_typed_threads mt' (empties threads') threads' /\
+    well_typed_memory mt' m'.
+Proof.
+  intros * Hthreads Hmem Hcstep. induction Hcstep.
+  - eauto using step_preserves_well_typed_threads.
+  - rewrite add_set_comm; trivial.
+    eapply step_preserves_well_typed_threads; eauto.
+    + unfold get_tm in *. rewrite get_add_lt; eauto.
+    + destruct (Hthreads i (empties_length threads)) as [T Htype].
+      rewrite empties_returns_empty in Htype.
+      assert (Hblock : exists B, mt / empty |-- block is B).
+      { eauto using spawn_block_has_type. }
+      destruct Hblock.
+      eauto using spawn_preserves_well_typed_threads, extends_refl.
+Qed.
+
+Theorem cprogress : forall threads m mt,
+  well_typed_memory mt m ->
+  well_typed_threads mt (empties threads) threads ->
+  (finished threads \/ exists m' threads', m / threads ==> m' / threads').
+Proof.
+  intros * Hmem Hth.
+  induction threads as [| th ths IH].
+  - left. intros i. destruct i; apply V_Nil.
+  - rewrite aux4 in Hth.
+    apply aux2 in Hth as Hth'.
+    specialize (IH Hth') as [IH | [m' [threads' IH]]].
+    + destruct (is_value th) eqn:E.
+      * left. apply value_equivalence in E.
+        intros i. destruct i; unfold get_tm; simpl; trivial.
+      * right.
+        specialize (Hth 0). simpl in Hth.
+        specialize (Hth (aux6 ths)) as [T Htype].
+        unfold get_ctx, get_tm in Htype. simpl in Htype.
+        assert (value th \/ exists m' th' eff, m / th --> eff / m' / th').
+        { eauto using progress. }
+        destruct H as [F | [m' [th' [eff Hstep]]]].
+        ** apply value_equivalence in F. rewrite E in F. discriminate.
+        ** destruct eff.
+          *** eexists. eexists. eauto using (CST_None 0).
+          *** eexists. eexists. eauto using (CST_Spawn 0), Nat.lt_0_succ.
+    + right. exists m'. exists (th :: threads'). eauto using aux5.
 Qed.
